---
title: "[Proof] Quadratic Formula"
date: "2025-01-07"
categories: [Math]
---

$$
\begin{align*}
&ax^2+bx+c=0 \ (a \neq 0) \\
&x^2+\frac{b}{a}x+\frac{c}{a}=0\\&(x+\frac{b}{2a})^2=-\frac{c}{a}+\frac{b^2}{4a^2}\\
&(x+\frac{b}{2a})^2=\frac{-4ac+b^2}{4a^2}\\
&x+\frac{b}{2a}=\pm\sqrt{\frac{b^2-4ac}{4a^2}}\\
&x=\pm\sqrt{\frac{b^2-4ac}{4a^2}}-\frac{b}{2a}\\
&x=\pm\frac{\sqrt{b^2-4ac}}{2a}-\frac{b}{2a}\\
&x=\frac{-b\pm\sqrt{b^2-4ac}}{2a}
\end{align*}
$$

Therefore,

-   If $b^2-4ac>0$, there are two real roots

-   If $b^2-4ac=0$, there is only one real root (or two repeated roots)

-   If $b^2-4ac<0$, there is no real root (or two complex conjugate root)